---
title: "COS4807 Assignment 1 - 791729"
author: "Christopher Deon Steenkamp - 36398934"
output: pdf_document
geometry: margin=1in
header-includes:
  - \usepackage{mathrsfs}
---
## Question 1

$$\begin{aligned}
(p \rightarrow q) \leftrightarrow (p \rightarrow r) &\equiv
\big((p \rightarrow q) \rightarrow (p \rightarrow r)\big)\land\big((p \rightarrow r) \rightarrow (p \rightarrow q)\big) &&\text{remove biconditional}\\
&\equiv \big(\neg (p \rightarrow q) \lor (p \rightarrow r)\big)\land\big(\neg(p \rightarrow r) \lor (p \rightarrow q)\big) &&\text{remove conditional} \\
&\equiv \big(\neg (\neg p \lor q) \lor (\neg p \lor r)\big)\land\big(\neg(\neg p \lor r) \lor (\neg p \lor q)\big) &&\text{remove conditional} \\
&\equiv \big((\neg\neg p \land\neg q) \lor (\neg p \lor r)\big)\land\big((\neg\neg p \land\neg r) \lor (\neg p \lor q)\big) &&\text{De Morgan} \\
&\equiv \big((p \land\neg q) \lor (\neg p \lor r)\big)\land\big((p \land\neg r) \lor (\neg p \lor q)\big) &&\text{remove } \neg\neg \\
&\equiv \big((p \lor \neg p \lor r) \land(\neg q \lor \neg p \lor r)\big)\land\big((p \lor \neg p \lor q) \land(\neg r\lor \neg p \lor q)\big) &&\text{distribute disjunction} \\
&\equiv (p \lor \neg p \lor r) \land(\neg q \lor \neg p \lor r)\land(p \lor \neg p \lor q) \land(\neg r\lor \neg p \lor q)
\end{aligned}
$$

In clausal form is:
$\{\{p,\neg p, r\},\{\neg q,\neg p, r\},\{p, \neg p, q\},\{\neg r, \neg p, q\}\}$

Without trivial clauses:
$\{\{\neg q,\neg p, r\},\{\neg r, \neg p, q\}\}$

Which can be abbreviated as:
$\{ \bar q\bar pr, \bar r\bar pq \}$

## Question 2

$$
\begin{aligned}
&\big((p\rightarrow q)\rightarrow\neg(r\rightarrow q)\big) \land \big((\neg r\rightarrow p)\rightarrow(p\rightarrow q)\big) \\
&\equiv \big(\neg(p\rightarrow q)\lor\neg(r\rightarrow q)\big) \land \big(\neg(\neg r\rightarrow p)\lor(p\rightarrow q)\big) \\
&\equiv \big(\neg(\neg p\lor q)\lor\neg(\neg r\lor q)\big) \land \big(\neg(\neg\neg r\lor p)\lor(\neg p\lor q)\big) \\
&\equiv \big((\neg\neg p\land\neg q)\lor(\neg\neg r\land\neg q)\big) \land \big((\neg\neg\neg r\land\neg p)\lor(\neg p\lor q)\big) \\
&\equiv \big((p\land\neg q)\lor(r\land\neg q)\big) \land \big((\neg r\land\neg p)\lor(\neg p\lor q)\big) \\
&\equiv (p\lor r)\land(p\lor \neg q)\land(\neg q\lor r)\land(\neg q\lor \neg q)\land(\neg r\lor\neg p\lor q)\land(\neg p\lor\neg p\lor q) \\
\end{aligned}
$$

In abbreviated clausal form:
$\{ pr,p\bar q,\bar qr,\bar q,\bar r\bar pq,\bar pq \}$

1. $pr$
1. $p\bar q$
1. $\bar qr$
1. $\bar q$
1. $\bar r\bar pq$
1. $\bar pq$
1. $rq\text{\space\space\space\space\space\space\space\space\space\space}$ 1,6
1. $r\bar p\text{\space\space\space\space\space\space\space\space\space\space}$ 3,6
1. $r\text{\space\space\space\space\space\space\space\space\space\space\space\space}$ 3,7
1. $\bar r\bar p\text{\space\space\space\space\space\space\space\space\space\space}$ 4,5
1. $\bar p\text{\space\space\space\space\space\space\space\space\space\space\space\space}$ 4,6
1. $r\bar q\text{\space\space\space\space\space\space\space\space\space\space}$ 2,8
1. $\bar q\bar r\text{\space\space\space\space\space\space\space\space\space\space}$ 2,9
1. $pr\text{\space\space\space\space\space\space\space\space\space\space}$ 2,7
1. $\bar q\bar p\text{\space\space\space\space\space\space\space\space\space\space}$ 3,9

Because we can resolve no new clauses and we have not attained a $\square$, we conclude that the formula is satisfiable.

## Question 3

Formula|Clausal Form
:-:|:-:
$p\rightarrow(q\lor r)$|$\bar pqr$
$(p\rightarrow r)\rightarrow q$|$pq, q\bar r$
$\neg q$|$\bar q$

We will use resolution to attain a $\square$ to show that the set of formulas where we have negated the goal are unsatisfiable.

1. $\bar pqr$
1. $pq$
1. $q\bar r$
1. $\bar q\text{\space\space\space\space\space\space\space\space\space\space\space\space}$ negation of goal
1. $qr \text{\space\space\space\space\space\space\space\space\space\space}$ 1,2
1. $q \text{\space\space\space\space\space\space\space\space\space\space\space\space}$ 3,5
1. $\square \text{\space\space\space\space\space\space\space\space\space\space\space}$ 4,6

We have proved that the set of clauses are unsatisfiable and so shown that the formulas from which they are derived are also unstatisfiable. Therefore, we conclude that $\{p\rightarrow(q\lor r), (p\rightarrow r)\rightarrow q\} \models q$

## Question 4

We wish to prove that if the set of clauses labeling the leaves of a resolution tree are satisfiable, then the clause at the root of the tree is satisfiable.

We show this by structural induction on the height of the tree.

Base Case: Let $C$ be an arbitrary clause which is satisfiable. Then, if the resolution tree is labeled by $C$ and has a height $n = 0$, $C$ is also a leaf node and so is, by definition, satisifiable.

Inductive Step: With $n > 0$ we have $C$ being formed by the resolution of two subtrees, $C_1$ and $C_2$ each with height $k < n$. Assume $C_1$ and $C_2$ are satisfiable under some interpretation $\mathscr{I}$. Since, for some complementary set of literals $l,l^c$, we have that either $\mathscr{I}(l)=T$ or $\mathscr{I}(l^c)=T$.

Suppose $\mathscr{I}(l)=T$, then $\mathscr{I}(l^c)=F$. If $l\in C_1$ then we have that $l^c\in C_2$ and so $C_2$ can be satisfied only by some other literal $l' \in C_2$ with $\mathscr{I}(l')=T$ (and $l' \neq l^c$). The resoultion rule defines $C = (C_1 - \{l\})\cup(C_2 - \{l^c\})$ so $l'\in C$ which means that $C$ is also satisfiable. A symmetric argument holds when $\mathscr{I}(l^c)=T$

## Question 5

### 5(i)

Given the following sudoku board with cells numbered $1 - 9$, we define the set of clauses required to encode the problem as follows:

$$
\def\arraystretch{1.5}
\begin{array}{|c|c|c|}
\hline
1 & 2 & 3 \\ \hline
4 & 5 & 6 \\ \hline
7 & 8 & 9 \\ \hline
\end{array}
$$

We encode the fact that each cell must contain at least one number as follows:
$$
\begin{aligned}
&11\lor12\lor13,\\
&21\lor22\lor23,\\
&31\lor32\lor33,\\
&41\lor42\lor43,\\
&51\lor52\lor53,\\
&61\lor62\lor63,\\
&71\lor72\lor73,\\
&81\lor82\lor83,\\
&91\lor92\lor93
\end{aligned}
$$

We add the constraint that a cell can contain at most one value:

$$
\begin{aligned}
&\overline{11}\lor\overline{12},\overline{11}\lor\overline{13},\overline{12}\lor\overline{13},\\
&\overline{21}\lor\overline{22},\overline{21}\lor\overline{23},\overline{22}\lor\overline{23},\\
&\overline{31}\lor\overline{32},\overline{31}\lor\overline{33},\overline{32}\lor\overline{33},\\
&\overline{41}\lor\overline{42},\overline{41}\lor\overline{43},\overline{42}\lor\overline{43},\\
&\overline{51}\lor\overline{52},\overline{51}\lor\overline{53},\overline{52}\lor\overline{53},\\
&\overline{61}\lor\overline{62},\overline{61}\lor\overline{63},\overline{62}\lor\overline{63},\\
&\overline{71}\lor\overline{72},\overline{71}\lor\overline{73},\overline{72}\lor\overline{73},\\
&\overline{81}\lor\overline{82},\overline{81}\lor\overline{83},\overline{82}\lor\overline{83},\\
&\overline{91}\lor\overline{92},\overline{91}\lor\overline{93},\overline{92}\lor\overline{93}
\end{aligned}
$$

Add the constraint that no two cells in a row can contain the same number:

$$
\begin{aligned}
&\overline{11}\lor\overline{21},\overline{12}\lor\overline{22},\overline{13}\lor\overline{23},\\
&\overline{11}\lor\overline{31},\overline{12}\lor\overline{32},\overline{13}\lor\overline{33},\\
&\overline{21}\lor\overline{31},\overline{22}\lor\overline{32},\overline{23}\lor\overline{33},\\
&\overline{41}\lor\overline{51},\overline{42}\lor\overline{52},\overline{43}\lor\overline{53},\\
&\overline{41}\lor\overline{61},\overline{42}\lor\overline{62},\overline{43}\lor\overline{63},\\
&\overline{51}\lor\overline{61},\overline{52}\lor\overline{62},\overline{53}\lor\overline{63},\\
&\overline{71}\lor\overline{81},\overline{72}\lor\overline{82},\overline{73}\lor\overline{83},\\
&\overline{71}\lor\overline{91},\overline{72}\lor\overline{92},\overline{73}\lor\overline{93},\\
&\overline{81}\lor\overline{91},\overline{82}\lor\overline{92},\overline{83}\lor\overline{93}
\end{aligned}
$$

And the constraint that no two cells in a column can contain the same number:

$$
\begin{aligned}
&\overline{11}\lor\overline{41},\overline{12}\lor\overline{42},\overline{13}\lor\overline{43},\\
&\overline{11}\lor\overline{71},\overline{12}\lor\overline{72},\overline{13}\lor\overline{73},\\
&\overline{41}\lor\overline{71},\overline{42}\lor\overline{72},\overline{43}\lor\overline{73},\\
&\overline{21}\lor\overline{51},\overline{22}\lor\overline{52},\overline{23}\lor\overline{53},\\
&\overline{21}\lor\overline{81},\overline{22}\lor\overline{82},\overline{23}\lor\overline{83},\\
&\overline{51}\lor\overline{81},\overline{52}\lor\overline{82},\overline{53}\lor\overline{83},\\
&\overline{31}\lor\overline{61},\overline{32}\lor\overline{62},\overline{33}\lor\overline{63},\\
&\overline{31}\lor\overline{91},\overline{32}\lor\overline{92},\overline{33}\lor\overline{93},\\
&\overline{61}\lor\overline{91},\overline{62}\lor\overline{92},\overline{63}\lor\overline{93}
\end{aligned}
$$

Finally we encode the given starting positions as unit clauses:

$12,61$

### 5(ii)

1. After applying unit propogation with $\mathscr{I}(12) = T$ we arrive at the following set of clauses:

    $$
    \begin{aligned}S= \{
    &21\lor23,\\
    &31\lor33,\\
    &41\lor43,\\
    &51\lor52\lor53,\\
    &61\lor62\lor63,\\
    &71\lor73,\\
    &81\lor82\lor83,\\
    &91\lor92\lor93,\\
    &\overline{21}\lor\overline{23},\\
    &\overline{31}\lor\overline{33},\\
    &\overline{41}\lor\overline{43},\\
    &\overline{51}\lor\overline{52},\overline{51}\lor\overline{53},\overline{52}\lor\overline{53},\\
    &\overline{61}\lor\overline{62},\overline{61}\lor\overline{63},\overline{62}\lor\overline{63},\\
    &\overline{71}\lor\overline{73},\\
    &\overline{81}\lor\overline{82},\overline{81}\lor\overline{83},\overline{82}\lor\overline{83},\\
    &\overline{91}\lor\overline{92},\overline{91}\lor\overline{93},\overline{92}\lor\overline{93},\\
    &\overline{21}\lor\overline{31},\overline{23}\lor\overline{33},\\
    &\overline{41}\lor\overline{51},\overline{43}\lor\overline{53},\\
    &\overline{41}\lor\overline{61},\overline{43}\lor\overline{63},\\
    &\overline{51}\lor\overline{61},\overline{52}\lor\overline{62},\overline{53}\lor\overline{63},\\
    &\overline{71}\lor\overline{81},\overline{73}\lor\overline{83},\\
    &\overline{71}\lor\overline{91},\overline{73}\lor\overline{93},\\
    &\overline{81}\lor\overline{91},\overline{82}\lor\overline{92},\overline{83}\lor\overline{93},\\
    &\overline{41}\lor\overline{71},\overline{43}\lor\overline{73},\\
    &\overline{21}\lor\overline{51},\overline{23}\lor\overline{53},\\
    &\overline{21}\lor\overline{81},\overline{23}\lor\overline{83},\\
    &\overline{51}\lor\overline{81},\overline{52}\lor\overline{82},\overline{53}\lor\overline{83},\\
    &\overline{31}\lor\overline{61},\overline{33}\lor\overline{63},\\
    &\overline{31}\lor\overline{91},\overline{33}\lor\overline{93},\\
    &\overline{61}\lor\overline{91},\overline{62}\lor\overline{92},\overline{63}\lor\overline{93}\}
    \end{aligned}
    $$
1. Setting $\mathscr{I}(61) = T$, and applying unit propogation to the resultant set of clauses $S$, we are able to resolve all the remaining clauses and are left with $S = \emptyset$.\
\
    We conclude that the initial set of clauses is satisfiable and take the solution to be valuations $\mathscr{I}(12)=T,\mathscr{I}(11)=F,\mathscr{I}(13)=F,\mathscr{I}(22)=F,\mathscr{I}(32)=F,\mathscr{I}(42)=F,\mathscr{I}(72)=F,\mathscr{I}(61)=T,\mathscr{I}(62)=F,\mathscr{I}(63)=F,\mathscr{I}(41)=F,\mathscr{I}(51)=F,\mathscr{I}(43)=T,\mathscr{I}(53)=F,\mathscr{I}(73)=F,\mathscr{I}(52)=T,\mathscr{I}(71)=T,\mathscr{I}(31)=F,\mathscr{I}(91)=F,\mathscr{I}(33)=T,\mathscr{I}(23)=F,\mathscr{I}(93)=F,\mathscr{I}(21)=T,\mathscr{I}(92)=T,\mathscr{I}(81)=F,\mathscr{I}(82)=F,\mathscr{I}(83)=T$\
\
    Which is the following solution\
    \
    $$
    \def\arraystretch{1.5}
    \begin{array}{|c|c|c|}
    \hline
    2 & 1 & 3 \\ \hline
    3 & 2 & 1 \\ \hline
    1 & 3 & 2 \\ \hline
    \end{array}
    $$
